Prove some more specs for helpers
Fix yet another bug in the process; [get_logwrite] was off-by-one,
caught by asymmetry with [set_desc] (the proof also would have failed).

src/Examples/Logging/Impl.v
@@ -145,7 +145,7 @@ Definition set_desc desc (i:nat) a v :=
 
 Definition get_logwrite desc (i:nat) :=
     let a := sel desc.(addresses) i in
-    v <- read (1+i);
+    v <- read (2+i);
       Ret (a, v).
 
 (* manipulating the data region *)
